implement JRH's term ordering and prove equivalent to current ACONV
I believe John Harrison's latest (or maybe it is in progress) kernel for
HOL Light uses a term ordering along the lines defined here (I am
copying definitions from him) to test terms for alpha-equivalence but
also to maintain sets with canonical representations as lists (by
sorting) for hypotheses on theorems.

The plan is eventually to use this ordering, or something like it, for
our model of the inference system too. This might also help with the
conservativity proof, where the order (and even duplicate elements) of
hypothesis list elements was causing problems. It will certainly help
with proving derived rules for our inference system.

Equivalence with the current ACONV is a sanity check on the definitions.
It might also be the basis for avoiding a lot of proof updating if the
inference system changes (but not sure if that will work out...).

hol-light/standard/syntax/holSyntaxScript.sml
@@ -87,6 +87,167 @@ val TERM_UNION_def = Define`
     let subun = TERM_UNION t l2 in
     if EXISTS (ACONV h) subun then subun else h::subun`
 
+(* Term ordering, respecting alpha-equivalence *)
+(* TODO: use this in the inference system instead of
+   ALPHAVARS, ACONV, TERM_UNION, etc., which don't
+   lead to canonical hypothesis sets-as-lists *)
+
+(* TODO: move, see HOL issue #219 *)
+local open pairTheory relationTheory in
+val LEX_CONG = store_thm("LEX_CONG",
+  ``(R1 x1 x2 <=> R1' x1' x2') /\
+    (~(R1 x1 x2) ==> ((x1 = x2) <=> (x1' = x2'))) /\
+    (~(R1 x1 x2) ==> (R2 y1 y2 <=> R2' y1' y2'))
+    ==> ((R1 LEX R2) (x1,y1) (x2,y2) <=> (R1' LEX R2') (x1',y1') (x2',y2'))``,
+  SRW_TAC[][LEX_DEF_THM] THEN METIS_TAC[])
+val () = DefnBase.export_cong"LEX_CONG"
+val LEX_MONO = store_thm("LEX_MONO",
+  ``(!x y. R1 x y ==> R2 x y) /\
+    (!x y. R3 x y ==> R4 x y)
+    ==>
+    (R1 LEX R3) x y ==> (R2 LEX R4) x y``,
+  STRIP_TAC THEN
+  Cases_on`x` THEN Cases_on`y` THEN
+  SRW_TAC[][LEX_DEF_THM] THEN
+  PROVE_TAC[])
+val () = IndDefLib.export_mono"LEX_MONO"
+end
+(* -- *)
+
+val (type_lt_rules,type_lt_ind,type_lt_cases) = Hol_reln`
+  (mlstring_lt x1 x2 ⇒ type_lt (Tyvar x1) (Tyvar x2)) ∧
+  (type_lt (Tyvar x1) (Tyapp x2 args2)) ∧
+  ((mlstring_lt LEX LIST_REL type_lt) (x1,args1) (x2,args2) ⇒
+     type_lt (Tyapp x1 args1) (Tyapp x2 args2))`
+
+val type_lt_thm = prove(
+  ``(type_lt (Tyvar x1) (Tyvar x2) ⇔ mlstring_lt x1 x2) ∧
+    (type_lt (Tyvar _) (Tyapp _ _) ⇔ T) ∧
+    (type_lt (Tyapp _ _) (Tyvar _) ⇔ F) ∧
+    (type_lt (Tyapp x1 args1) (Tyapp x2 args2) ⇔
+       (mlstring_lt LEX LIST_REL type_lt)
+         (x1,args1) (x2,args2))``,
+  rw[] >> rw[Once type_lt_cases])
+  |> CONJUNCTS |> map GEN_ALL |> LIST_CONJ
+  |> curry save_thm "type_lt_thm"
+
+val (term_lt_rules,term_lt_ind,term_lt_cases) = Hol_reln`
+  ((mlstring_lt LEX type_lt) (x1,ty1) (x2,ty2) ⇒
+    term_lt (Var x1 ty1) (Var x2 ty2)) ∧
+  (term_lt (Var x1 ty1) (Const x2 ty2)) ∧
+  (term_lt (Var x1 ty1) (Comb t1 t2)) ∧
+  (term_lt (Var x1 ty1) (Abs t1 t2)) ∧
+  ((mlstring_lt LEX type_lt) (x1,ty1) (x2,ty2) ⇒
+    term_lt (Const x1 ty1) (Const x2 ty2)) ∧
+  (term_lt (Const x1 ty1) (Comb t1 t2)) ∧
+  (term_lt (Const x1 ty1) (Abs t1 t2)) ∧
+  ((term_lt LEX term_lt) (s1,s2) (t1,t2) ⇒
+   term_lt (Comb s1 s2) (Comb t1 t2)) ∧
+  (term_lt (Comb s1 s2) (Abs t1 t2)) ∧
+  ((term_lt LEX term_lt) (s1,s2) (t1,t2) ⇒
+   term_lt (Abs s1 s2) (Abs t1 t2))`
+
+val term_lt_thm = prove(``
+  (term_lt (Var x1 ty1) (Var x2 ty2) ⇔
+     (mlstring_lt LEX type_lt) (x1,ty1) (x2,ty2)) ∧
+  (term_lt (Var _ _) (Const _ _) ⇔ T) ∧
+  (term_lt (Var _ _) (Comb _ _) ⇔ T) ∧
+  (term_lt (Var _ _) (Abs _ _) ⇔ T) ∧
+  (term_lt (Const _ _) (Var _ _) ⇔ F) ∧
+  (term_lt (Const x1 ty1) (Const x2 ty2) ⇔
+     (mlstring_lt LEX type_lt) (x1,ty1) (x2,ty2)) ∧
+  (term_lt (Const _ _) (Comb _ _) ⇔ T) ∧
+  (term_lt (Const _ _) (Abs _ _) ⇔ T) ∧
+  (term_lt (Comb _ _) (Var _ _) ⇔ F) ∧
+  (term_lt (Comb _ _) (Const _ _) ⇔ F) ∧
+  (term_lt (Comb s1 s2) (Comb t1 t2) ⇔
+     (term_lt LEX term_lt) (s1,s2) (t1,t2)) ∧
+  (term_lt (Comb _ _) (Abs _ _) ⇔ T) ∧
+  (term_lt (Abs _ _) (Var _ _) ⇔ F) ∧
+  (term_lt (Abs _ _) (Const _ _) ⇔ F) ∧
+  (term_lt (Abs _ _) (Comb _ _) ⇔ F) ∧
+  (term_lt (Abs s1 s2) (Abs t1 t2) ⇔
+    (term_lt LEX term_lt) (s1,s2) (t1,t2))``,
+  rw[] >> rw[Once term_lt_cases])
+  |> CONJUNCTS |> map GEN_ALL |> LIST_CONJ
+  |> curry save_thm "term_lt_thm"
+
+val _ = Datatype`order = LESS | EQUAL | GREATER`
+
+val lt_to_cmp_def = Define`
+  lt_to_cmp lt x y =
+    if x = y then EQUAL else
+    if lt x y then LESS else GREATER`
+
+val term_cmp_def = Define`
+  term_cmp = lt_to_cmp term_lt`
+
+val type_cmp_def = Define`
+  type_cmp = lt_to_cmp type_lt`
+
+val ordav_def = Define`
+  (ordav [] x1 x2 ⇔ term_cmp x1 x2) ∧
+  (ordav ((t1,t2)::env) x1 x2 ⇔
+    if term_cmp x1 t1 = EQUAL then
+      if term_cmp x2 t2 = EQUAL then
+        EQUAL
+      else LESS
+    else if term_cmp x2 t2 = EQUAL then
+      GREATER
+    else ordav env x1 x2)`
+
+val orda_def = Define`
+  orda env t1 t2 =
+    if t1 = t2 ∧ env = [] then EQUAL else
+      case (t1,t2) of
+      | (Var _ _, Var _ _) => ordav env t1 t2
+      | (Const _ _, Const _ _) => term_cmp t1 t2
+      | (Comb s1 t1, Comb s2 t2) =>
+        (let c = orda env s1 s2 in
+           if c ≠ EQUAL then c else orda env t1 t2)
+      | (Abs s1 t1, Abs s2 t2) =>
+        (let c = type_cmp (typeof s1) (typeof s2) in
+           if c ≠ EQUAL then c else orda ((s1,s2)::env) t1 t2)
+      | (Var _ _, _) => LESS
+      | (_, Var _ _) => GREATER
+      | (Const _ _, _) => LESS
+      | (_, Const _ _) => GREATER
+      | (Comb _ _, _) => LESS
+      | (_, Comb _ _) => GREATER`
+
+val term_union_def = Define`
+  term_union l1 l2 =
+    if l1 = l2 then l1 else
+    case (l1,l2) of
+    | ([],l2) => l2
+    | (l1,[]) => l1
+    | (h1::t1,h2::t2) =>
+      let c = orda [] h1 h2 in
+      if c = EQUAL then h1::(term_union t1 t2)
+      else if c = LESS then h1::(term_union t1 l2)
+      else h2::(term_union (h1::t1) t2)`
+
+val term_remove_def = Define`
+  term_remove t l =
+  case l of
+  | [] => l
+  | (s::ss) =>
+    let c = orda [] t s in
+    if c = GREATER then
+      let ss' = term_remove t ss in
+      if ss' = ss then l else s::ss'
+    else if c = EQUAL then ss else l`
+
+val term_image_def = Define`
+  term_image f l =
+  case l of
+  | [] => l
+  | (h::t) =>
+    let h' = f h in
+    let t' = term_image f t in
+    if h' = h ∧ t' = t then l
+    else term_union [h'] t'`
+
 (* Whether a variables (or constant) occurs free in a term. *)
 
 val VFREE_IN_def = Define`
